Use exp.lam' to bind name in patterns

src/exp/type.lean
@@ -10,7 +10,6 @@ namespace acie -----------------------------------------------------------------
 
 variables {V : Type} [decidable_eq V] -- Type of variable names
 variables {vs : Type → Type} [vset vs V] -- Type of variable name sets
-variables {X : vs V} -- Variable name sets
 
 /-
 `exp` is an inductive data type representing a lambda calculus expression
@@ -22,5 +21,12 @@ inductive exp : vs V → Type
   | var : Π {X : vs V},         ν∈ X             → exp X  -- variable
   | app : Π {X : vs V},         exp X → exp X    → exp X  -- application
   | lam : Π {X : vs V} {a : V}, exp (insert a X) → exp X  -- lambda abstraction
+
+variables {X : vs V} -- Variable name sets
+
+-- A utility pattern for binding the name.
+@[pattern, reducible]
+def exp.lam' (a : V) : exp (insert a X) → exp X :=
+  @exp.lam _ _ _ _ _ a
 
 end /- namespace -/ acie -------------------------------------------------------
